All the recent stuff. Defined Binary Random-Access Lists using Structural Decomposition. Moved a few things from BST to BTree. Proved a lot of stuff about Splay Heaps. Improved splaySort's performance significantly and proved that it sorts. Defined alternative Splay Heaps using smaller and bigger (as in the exercise). Proved lots of things about pairing heaps and proved that pairingSort sorts.

DS/BST.v
@@ -13,7 +13,7 @@ Inductive is_bst {A : LinDec} : BTree A -> Prop :=
         (forall x : A, elem x r -> leq v x) -> is_bst r ->
         is_bst (node v l r).
 
-Hint Constructors BTree elem is_bst.
+Hint Constructors elem is_bst.
 
 Lemma is_bst_inv_l : forall (A : LinDec) (v : A) (l r : BTree A),
     is_bst (node v l r) -> is_bst l.
@@ -48,6 +48,12 @@ Proof.
     1-2: by [].
     move: (H5 _ H9) => H'. have Heq : x = v by eapply leq_antisym.
       contradiction.
+Restart.
+  intros. inv H. inv H0.
+    contradiction.
+    specialize (H8 _ H3). assert (x = v).
+      apply leq_antisym; auto.
+      subst. contradiction.
 Qed.
 
 Lemma is_bst_inv_elem_r :
@@ -60,6 +66,12 @@ Proof.
     move: (H3 _ H9) => H'. have Heq : x = v by eapply leq_antisym.
       contradiction.
     by [].
+Restart.
+  intros. inv H. inv H0.
+    contradiction.
+    specialize (H6 _ H3). assert (x = v).
+      apply leq_antisym; auto.
+      subst. contradiction.
 Qed.
 
 Hint Resolve is_bst_inv_l is_bst_inv_r.
@@ -120,8 +132,8 @@ Proof.
       case: (elem_ins _ _ _ _ Helt) => [-> |]; eauto.
 Qed.
 
-Fixpoint min {A : Type} (bta : BTree A) : option A :=
-match bta with
+Fixpoint min {A : Type} (t : BTree A) : option A :=
+match t with
     | empty => None
     | node v empty _ => Some v
     | node _ l _ => min l
@@ -160,48 +172,15 @@ Proof.
         apply H7. assumption.
 Qed.
 
-(* toList, fromList and their variants *)
-Function toList {A : Type} (t : BTree A) : list A :=
-match t with
-    | empty => []
-    | node v l r => toList l ++ v :: toList r
-end.
-
+(** [fromList] and its variants. *)
 Function fromList (A : LinDec) (l : list A) : BTree A :=
 match l with
     | [] => empty
     | h :: t => BTree_ins h (fromList A t)
 end.
 
-Function toList'_aux {A : LinDec} (t : BTree A) (acc : list A) : list A :=
-match t with
-    | empty => acc
-    | node v l r => toList'_aux l (v :: toList'_aux r acc)
-end.
-
-Definition toList' {A : LinDec} (t : BTree A) : list A :=
-  toList'_aux t [].
-
 Definition fromList' {A : LinDec} (l : list A) : BTree A :=
   fold_left (fun t x => BTree_ins x t) l empty.
-
-(* Counting elements in a binary tree. *)
-Fixpoint count_BTree (A : LinDec) (x : A) (t : BTree A) : nat :=
-match t with
-    | empty => 0
-    | node v l r =>
-        let n := count_BTree A x l in
-        let m := count_BTree A x r in
-        if x =? v then S (n + m) else n + m
-end.
-
-Lemma count_toList :
-  forall (A : LinDec) (x : A) (t : BTree A),
-    count A x (toList t) = count_BTree A x t.
-Proof.
-  intros. elim: t x => [| v l Hl r Hr] //= x.
-    by dec; rewrite count_app Hl //= Hr; dec.
-Qed.
 
 Lemma count_ins :
   forall (A : LinDec) (x h : A) (t : BTree A),
@@ -211,24 +190,6 @@ Lemma count_ins :
       else count_BTree A x t.
 Proof.
   intros. elim: t => [| v l Hl r Hr] //=; repeat dec.
-Qed.
-
-(* Lemmas for toList and others. *)
-Lemma toList'_aux_spec :
-  forall (A : LinDec) (t : BTree A) (acc : list A),
-    toList'_aux t acc = toList t ++ acc.
-Proof.
-  intros. functional induction @toList'_aux A t acc; cbn.
-    trivial.
-    rewrite <- app_assoc. cbn. rewrite <- IHl, <- IHl0. trivial.
-Qed.
-
-Require Import FunctionalExtensionality.
-
-Theorem toList'_spec : @toList' = @toList.
-Proof.
-  extensionality A. extensionality t. unfold toList'.
-  rewrite toList'_aux_spec app_nil_r. trivial.
 Qed.
 
 Function merge {A : LinDec} (t1 t2 : BTree A) : BTree A :=
@@ -264,32 +225,24 @@ Proof.
     fold fromList'.
 Abort.
 
-Lemma toList_In_elem :
-  forall (A : Type) (x : A) (t : BTree A),
-    In x (toList t) <-> elem x t.
-Proof.
-  split.
-    elim: t x => [| v l Hl r Hr] x H.
-      inversion H.
-      cbn in H. apply in_app_or in H. do 2 (destruct H; subst; auto).
-    elim: t x => [| v l Hl r Hr] x H //=; inversion H; subst;
-    apply in_or_app; cbn; eauto.
-Qed.
-
-Require Import RCCBase.
-
-Theorem toList_sorted :
+Theorem BTree_toList_sorted :
   forall (A : LinDec) (t : BTree A),
-    is_bst t -> sorted A (@toList (@carrier A) t).
+    is_bst t -> sorted A (@BTree_toList (@carrier A) t).
 Proof.
   induction t as [| v l Hl r Hr]; cbn; intros.
     constructor.
     inv H. apply sorted_app_all; auto.
-      case_eq (toList r); intros; subst; auto.
-        constructor.
-          apply H5. rewrite <- toList_In_elem. rewrite H. cbn. auto.
-          rewrite <- H. auto.
+      case_eq (BTree_toList r); intros; subst; auto. constructor.
+        apply H5. rewrite <- toList_In_elem. rewrite H. cbn. auto.
+        rewrite <- H. auto.
       intros. apply toList_In_elem in H. auto.
+Qed.
+
+Theorem toList'_sorted :
+  forall (A : LinDec) (t : BTree A),
+    is_bst t -> sorted A (toList' t).
+Proof.
+  rewrite toList'_spec. apply BTree_toList_sorted.
 Qed.
 
 Lemma fromList_is_bst :
@@ -297,13 +250,6 @@ Lemma fromList_is_bst :
 Proof.
   intros. elim: l => [| h t IH] //=.
     by apply BTree_ins_is_bst.
-Qed.
-
-Theorem toList'_sorted :
-  forall (A : LinDec) (t : BTree A),
-    is_bst t -> sorted A (toList' t).
-Proof.
-  rewrite toList'_spec. apply toList_sorted.
 Qed.
 
 Lemma fromList'_is_bst :
