DS/BTree.v
@@ -1,19 +1,20 @@
-Require Import Coq.Program.Wf.
-Require Export Compare_dec.
-Require Export Arith.
+Add Rec LoadPath "/home/zeimer/Code/Coq".
+
+Require Import RCCBase.
+
+Require Import LinDec.
+Require Import ListLemmas.
+Require Import Sorting.Sort.
+
 Require Export Classes.EquivDec.
-
-Require Import List.
-Import ListNotations.
-
-Set Implicit Arguments.
+Require Export Compare_dec.
 
 Inductive BTree (A : Type) : Type :=
     | empty : BTree A
     | node : A -> BTree A -> BTree A -> BTree A.
 
-Arguments empty [A].
-Arguments node [A] _ _ _.
+Arguments empty {A}.
+Arguments node {A} _ _ _.
 
 Fixpoint size {A : Type} (bt : BTree A) : nat :=
 match bt with
@@ -40,31 +41,28 @@ match bt with
     | node v l r => node (f v) (map f l) (map f r)
 end.
 
-From mathcomp Require Import ssreflect.
+(*From mathcomp Require Import ssreflect.*)
 
 Theorem map_pres_size : forall (A B : Type) (f : A -> B) (bt : BTree A),
     size bt = size (map f bt).
 Proof.
-  induction bt as [| v l Hl r Hr]; intros.
-    trivial.
-    simpl. f_equal. rewrite <- Hl, <- Hr. trivial.
-Restart.
-  intros. elim: bt => //= v l -> r -> //=. 
+  induction bt as [| v l Hl r Hr]; cbn; intros;
+  rewrite <- ?Hl, <- ?Hr; reflexivity.
+(*Restart.
+  intros. elim: bt => //= v l -> r -> //=. *)
 Qed.
 
-Fixpoint combine {A B : Type} (ta : BTree A) (tb : BTree B)
-    : BTree (A * B) :=
+Fixpoint combine
+  {A B : Type} (ta : BTree A) (tb : BTree B) : BTree (A * B) :=
 match ta, tb with
     | empty, _ => empty
     | _, empty => empty
-    | node v1 l1 r1, node v2 l2 r2 => node (v1, v2) (combine l1 l2) (combine r1 r2)
+    | node v1 l1 r1, node v2 l2 r2 =>
+        node (v1, v2) (combine l1 l2) (combine r1 r2)
 end.
 
-Definition l1 := [3; 0; 1; 34; 19; 44; 21; 65; 5].
-Definition l2 := [4; 6; 0; 99; 3; 12].
-
-Fixpoint fold {A B : Set} (op : A -> B -> B -> B) (b : B) (bt : BTree A)
-  : B :=
+Fixpoint fold
+  {A B : Set} (op : A -> B -> B -> B) (b : B) (bt : BTree A) : B :=
 match bt with
     | empty => b
     | node v l r => op v (fold op b l) (fold op b r)
@@ -85,18 +83,6 @@ Definition count_fold (n : nat) : BTree nat -> nat :=
 Definition map_fold {A B : Set} (f : A -> B) : BTree A -> BTree B :=
     fold (fun v l r => node (f v) l r) empty.
 
-(*Definition t1 : BTree nat := fromList leb l1.
-
-Eval compute in l1.
-Eval compute in sizegth l1.
-Eval compute in t1.
-Eval compute in map (fun x => x + 1) t1.
-Eval compute in map_fold (fun x => x + 1) t1.
-Eval compute in size_fold t1.
-Eval compute in sum_fold t1.
-Eval compute in find_fold 0 t1.
-Eval compute in count_fold 0 t1.*)
-
 Inductive elem {A : Type} (a : A) : BTree A -> Prop :=
     | elem_root : forall l r : BTree A, elem a (node a l r)
     | elem_left : forall (v : A) (l r : BTree A),
@@ -111,18 +97,98 @@ Theorem elem_dec :
     {elem a t} + {~ elem a t}.
 Proof.
   induction t as [| v l IHl r IHr].
-    right. intro. inversion H.
-    case (dec a v); intro.
+    right. inversion 1.
+    destruct (dec a v).
       left. rewrite <- e. constructor.
       destruct IHl as [IHl1 | IHl2].
         left. apply elem_left. assumption.
         destruct IHr as [IHr1 | IHr2].
           left. apply elem_right; assumption.
           right. intro. inversion H; contradiction.
-Restart.
+(*Restart.
   intros. elim: t => [| v l [Hl | Hl] r [Hr | Hr]]; auto.
     right. inversion 1.
     case: (dec a v) => H; [left | right].
       by rewrite H.
-      by inversion 1.
+      by inversion 1.*)
 Defined.
+
+Fixpoint elem_decb
+  {A : Type} (dec : EqDec A eq) (x : A) (t : BTree A) : bool :=
+match t with
+    | empty => false
+    | node v l r =>
+        if dec x v
+        then true
+        else elem_decb dec x l || elem_decb dec x r
+end.
+
+Require Import Bool.
+
+Lemma elem_decb_reflect :
+  forall (A : Type) (dec : EqDec A eq) (x : A) (t : BTree A),
+    reflect (elem x t) (elem_decb dec x t).
+Proof.
+  induction t as [| v l IHl r IHr]; cbn.
+    constructor. inversion 1.
+    destruct (dec x v), IHl, IHr; try inv e; cbn; auto.
+      constructor. intro. inv H. contradiction c. reflexivity.
+Qed.
+
+(* toList, fromList and their variants *)
+Function BTree_toList {A : Type} (t : BTree A) : list A :=
+match t with
+    | empty => []
+    | node v l r => BTree_toList l ++ v :: BTree_toList r
+end.
+
+Function toList'_aux {A : LinDec} (t : BTree A) (acc : list A) : list A :=
+match t with
+    | empty => acc
+    | node v l r => toList'_aux l (v :: toList'_aux r acc)
+end.
+
+Definition toList' {A : LinDec} (t : BTree A) : list A :=
+  toList'_aux t [].
+
+Lemma toList'_aux_spec :
+  forall (A : LinDec) (t : BTree A) (acc : list A),
+    toList'_aux t acc = BTree_toList t ++ acc.
+Proof.
+  intros. functional induction @toList'_aux A t acc; cbn.
+    trivial.
+    rewrite <- app_assoc. cbn. rewrite <- IHl, <- IHl0. trivial.
+Qed.
+
+Theorem toList'_spec : @toList' = @BTree_toList.
+Proof.
+  ext A. ext t. unfold toList'.
+  rewrite toList'_aux_spec, app_nil_r. trivial.
+Qed.
+
+(* Counting elements in a binary tree. *)
+Fixpoint count_BTree (A : LinDec) (x : A) (t : BTree A) : nat :=
+match t with
+    | empty => 0
+    | node v l r =>
+        let n := count_BTree A x l in
+        let m := count_BTree A x r in
+        if x =? v then S (n + m) else n + m
+end.
+
+Lemma count_toList :
+  forall (A : LinDec) (x : A) (t : BTree A),
+    count A x (BTree_toList t) = count_BTree A x t.
+Proof.
+  induction t; cbn; rewrite ?count_app; dec.
+Qed.
+
+Lemma toList_In_elem :
+  forall (A : Type) (x : A) (t : BTree A),
+    In x (BTree_toList t) <-> elem x t.
+Proof.
+  split.
+    induction t; cbn; intros; try apply in_app_or in H; firstorder.
+      subst. firstorder.
+    induction 1; cbn; firstorder.
+Qed.
