DS/PairingHeap.v
@@ -1,7 +1,7 @@
 Add Rec LoadPath "/home/zeimer/Code/Coq".
 
 Require Export LinDec.
-Require Import Sorting.Sort.
+Require Export RCCBase.
 
 Set Implicit Arguments.
 
@@ -38,17 +38,68 @@ Proof.
   induction t using Tree_rect' with (Q := Forall P); auto.
 Qed.
 
+Theorem Tree_ind_proper'
+  (A : Type) (P : Tree A -> Prop)
+  (HE : P E)
+  (Hnil : forall x : A, P (T x []))
+  (HT : forall (x : A) (t : Tree A) (l : list (Tree A)),
+    P t -> Forall P l -> P (T x (t :: l)))
+  (t : Tree A) : P t.
+Proof.
+  induction t using Tree_ind_proper; auto.
+  destruct l.
+    apply Hnil.
+    apply HT; inv H.
+Qed.
+
+Inductive elem {A : Type} (x : A) : Tree A -> Prop :=
+    | elem0 : forall l : list (Tree A), elem x (T x l)
+    | elem1 : forall (a : A) (l : list (Tree A)),
+        Exists (fun t => elem x t) l -> elem x (T a l).
+
+Inductive isHeap {A : LinDec} : Tree A -> Prop :=
+    | isHeap_E : isHeap E
+    | isHeap_T :
+        forall (v : A) (l : list (Tree A)),
+          Forall (fun t : Tree A => forall x : A, elem x t -> v ≤ x) l ->
+          Forall (fun t : Tree A => isHeap t) l ->
+            isHeap (T v l).
+
+Lemma isHeap_inv :
+  forall (A : LinDec) (x : A) (l : list (Tree A)),
+    isHeap (T x l) -> Forall isHeap l.
+Proof.
+  intros. inv H.
+Qed.
+
+Lemma isHeap_inv' :
+  forall (A : LinDec) (v : A) (l : list (Tree A)),
+    isHeap (T v l) ->
+      Forall (fun t : Tree A => forall x : A, elem x t -> v ≤ x) l.
+Proof.
+  intros. inv H.
+Qed.
+
+Hint Constructors elem isHeap.
+
 Definition PairingHeap (A : LinDec) : Type := Tree A.
 
 Definition empty {A : LinDec} : PairingHeap A := E.
 
+Definition isEmpty
+  {A : LinDec} (h : PairingHeap A) : bool :=
+match h with
+    | E => true
+    | _ => false
+end.
+
 Definition singleton {A : LinDec} (x : A) : PairingHeap A := T x [].
 
-Definition findMin {A : LinDec} (h : PairingHeap A) : option A :=
+(*Definition findMin {A : LinDec} (h : PairingHeap A) : option A :=
 match h with
     | E => None
     | T m _ => Some m
-end.
+end.*)
 
 Definition merge
   {A : LinDec} (h1 h2 : PairingHeap A) : PairingHeap A :=
@@ -73,9 +124,477 @@ match hs with
     | h1 :: h2 :: hs' => merge (merge h1 h2) (mergePairs hs')
 end.
 
-Definition deleteMin {A : LinDec} (h : PairingHeap A)
-  : PairingHeap A :=
+(*Definition deleteMin' {A : LinDec} (h : PairingHeap A)
+  : option (PairingHeap A) :=
 match h with
-    | E => E
-    | T _ hs => mergePairs hs
+    | E => None
+    | T _ hs => Some (mergePairs hs)
+end.*)
+
+(* TODO: develop *)
+Definition unT
+  {A : LinDec} (h : PairingHeap A) : option (A * PairingHeap A) :=
+match h with
+    | E => None
+    | T x l => Some (x, mergePairs l)
 end.
+
+Fixpoint size {A : Type} (t : Tree A) : nat :=
+match t with
+    | E => 0
+    | T _ ts => 1 + fold_right (fun h t => size h + t) 0 ts
+end.
+
+(** Properties of [empty] and [isEmpty]. *)
+
+Lemma empty_elem :
+  forall (A : LinDec) (x : A), ~ elem x empty.
+Proof. inversion 1. Qed.
+
+Lemma isEmpty_elem :
+  forall (A : LinDec) (x : A) (h : PairingHeap A),
+    isEmpty h = true -> ~ elem x h.
+Proof.
+  destruct h; cbn; intro.
+    inversion 1.
+    congruence.
+Qed.
+
+Lemma empty_isHeap :
+  forall A : LinDec, isHeap (@empty A).
+Proof. constructor. Qed.
+
+Lemma isEmpty_isHeap :
+  forall (A : LinDec) (h : PairingHeap A),
+    isEmpty h = true -> isHeap h.
+Proof.
+  destruct h; cbn; intro.
+    constructor.
+    congruence.
+Qed.
+
+Lemma isEmpty_empty :
+  forall A : LinDec, isEmpty (@empty A) = true.
+Proof. reflexivity. Qed.
+
+Lemma isEmpty_singleton :
+  forall (A : LinDec) (x : A),
+    isEmpty (singleton x) = false.
+Proof. reflexivity. Qed.
+
+Lemma isEmpty_merge :
+  forall (A : LinDec) (h1 h2 : PairingHeap A),
+    isEmpty (merge h1 h2) = isEmpty h1 && isEmpty h2.
+Proof.
+  destruct h1, h2; cbn; dec.
+Qed.
+
+Lemma isEmpty_merge_true :
+  forall (A : LinDec) (h1 h2 : PairingHeap A),
+    isEmpty (merge h1 h2) = true <->
+    isEmpty h1 = true /\ isEmpty h2 = true.
+Proof.
+  split; destruct h1, h2; cbn; intros; destruct H; dec.
+Qed.
+
+Lemma isEmpty_merge_false :
+  forall (A : LinDec) (h1 h2 : PairingHeap A),
+    isEmpty (merge h1 h2) = false <->
+    isEmpty h1 = false \/ isEmpty h2 = false.
+Proof.
+  split; destruct h1, h2; cbn; intros; destruct H; dec.
+Qed.
+
+Lemma isEmpty_insert :
+  forall (A : LinDec) (x : A) (h : PairingHeap A),
+    isEmpty (insert x h) = false.
+Proof.
+  destruct h; cbn; dec.
+Qed.
+
+Lemma isEmpty_size_false :
+  forall (A : LinDec) (t : Tree A),
+    isEmpty t = false -> size t <> 0.
+Proof.
+  destruct t; cbn; intro.
+    congruence.
+    inversion 1.
+Qed.
+
+Lemma isEmpty_size_true :
+  forall (A : LinDec) (t : Tree A),
+    isEmpty t = true -> size t = 0.
+Proof.
+  destruct t; cbn; intros.
+    reflexivity.
+    congruence.
+Qed.
+
+(** Properties of [singleton]. *)
+
+Lemma singleton_elem :
+  forall (A : LinDec) (x y : A),
+    elem x (singleton y) <-> x = y.
+Proof.
+  split; intro; subst.
+    inv H. inv H1.
+    constructor.
+Qed.
+
+Lemma singleton_elem' :
+  forall (A : LinDec) (x : A),
+    elem x (singleton x).
+Proof.
+  intros. rewrite singleton_elem. reflexivity.
+Qed.
+
+Lemma singleton_isHeap :
+  forall (A : LinDec) (x : A),
+    isHeap (singleton x).
+Proof. do 2 constructor. Qed.
+
+Lemma singleton_size :
+  forall (A : LinDec) (x : A),
+    size (singleton x) = 1.
+Proof. reflexivity. Qed.
+
+(** Properties of [merge]. *)
+
+Lemma merge_elem :
+  forall (A : LinDec) (x : A) (h1 h2 : PairingHeap A),
+    elem x (merge h1 h2) <-> elem x h1 \/ elem x h2.
+Proof.
+  split; destruct h1, h2; cbn; intros; dec; inv H; try inv H0; try inv H1.
+Qed.
+
+Lemma merge_isHeap :
+  forall (A : LinDec) (h1 h2 : PairingHeap A),
+    isHeap h1 -> isHeap h2 -> isHeap (merge h1 h2).
+Proof.
+  destruct h1, h2; cbn; intros; auto. dec; do 2 constructor.
+    apply isHeap_inv' in H0. induction H0; intros.
+      inv H0. inv H2.
+      inv H2. inv H4. eauto.
+    inv H.
+    assumption.
+    inv H.
+    apply isHeap_inv' in H. induction H; intros.
+      inv H. inv H2.
+      inv H2. inv H4. eauto.
+    inv H0.
+    assumption.
+    inv H0.
+Restart.
+  destruct h1, h2; cbn; intros; auto.
+  dec; do 2 constructor; try (inv H; inv H0; fail).
+    inv H0. clear H4. induction H3; intros.
+      inv H0. inv H2.
+      inv H1. inv H4. eauto.
+    inv H. clear H4. induction H3; intros.
+      inv H. inv H2.
+      inv H1. inv H4. eauto.
+Qed.
+
+Lemma merge_size :
+  forall (A : LinDec) (h1 h2 : PairingHeap A),
+    size (merge h1 h2) = size h1 + size h2.
+Proof.
+  destruct h1, h2; cbn; intros; dec.
+Qed.
+
+(** Properties of [insert]. *)
+
+Lemma insert_isHeap :
+  forall (A : LinDec) (x : A) (h : PairingHeap A),
+    isHeap h -> isHeap (insert x h).
+Proof.
+  intros. unfold insert. apply merge_isHeap.
+    apply singleton_isHeap.
+    assumption.
+Qed.
+
+Lemma insert_elem :
+  forall (A : LinDec) (x y : A) (h : PairingHeap A),
+    elem x (insert y h) <-> x = y \/ elem x h.
+Proof.
+  unfold insert. split; intro.
+    apply merge_elem in H. destruct H; [left | right].
+      rewrite <- singleton_elem. assumption.
+      assumption.
+    rewrite merge_elem. inv H. left. apply singleton_elem'.
+Qed.
+
+Lemma insert_size :
+  forall (A : LinDec) (x : A) (h : PairingHeap A),
+    size (insert x h) = 1 + size h.
+Proof.
+  destruct h; cbn; dec.
+Qed.
+
+(** Properties of [mergePairs]. *)
+
+Hint Extern 0 =>
+match goal with
+    | H : elem _ E |- _ => inv H
+    | H : elem _ empty |- _ => inv H
+end.
+
+Lemma mergePairs_elem :
+  forall (A : LinDec) (x : A) (l : list (Tree A)),
+    elem x (mergePairs l) <-> Exists (elem x) l.
+Proof.
+  split; intro.
+    functional induction @mergePairs A l; auto.
+      rewrite ?merge_elem in H. decompose [or] H; clear H; auto.
+    functional induction @mergePairs A l.
+      inv H.
+      inv H. inv H1.
+      rewrite ?merge_elem. inv H. inv H1.
+Qed.
+
+Lemma mergePairs_isHeap :
+  forall (A : LinDec) (l : list (PairingHeap A)),
+    Forall isHeap l -> isHeap (mergePairs l).
+Proof.
+  intros. functional induction @mergePairs A l.
+    constructor.
+    inv H.
+    inv H. inv H3. apply merge_isHeap.
+      apply merge_isHeap; assumption.
+      apply IHp. assumption.
+Qed.
+
+Lemma mergePairs_isEmpty :
+  forall (A : LinDec) (l : list (PairingHeap A)),
+    isEmpty (mergePairs l) = true <->
+    Forall (fun t => isEmpty t = true) l.
+Proof.
+  split.
+    functional induction @mergePairs A l; cbn; intros; auto.
+      rewrite ?isEmpty_merge_true in H. decompose [and] H. auto.
+    functional induction @mergePairs A l; cbn; intros; auto.
+      inv H.
+      rewrite ?isEmpty_merge_true. inv H. inv H3.
+Qed.
+
+Lemma mergePairs_size :
+  forall (A : LinDec) (l : list (PairingHeap A)),
+    size (mergePairs l) = fold_right (fun h t => size h + t) 0 l.
+Proof.
+  intros. functional induction @mergePairs A l; cbn; intros; auto.
+  rewrite !merge_size, IHp, plus_assoc. reflexivity.
+Qed.
+
+(** Properties of [unT]. *)
+
+Lemma unT_isHeap :
+  forall (A : LinDec) (m : A) (h h' : PairingHeap A),
+    isHeap h -> unT h = Some (m, h') -> isHeap h'.
+Proof.
+  destruct h; cbn; intros; subst; inv H0.
+  apply mergePairs_isHeap. inv H.
+Qed.
+
+Lemma unT_elem :
+  forall (A : LinDec) (m : A) (h h' : Tree A),
+    unT h = Some (m, h') -> elem m h.
+Proof.
+  destruct h; cbn; intros; inv H.
+Qed.
+
+Lemma unT_size :
+  forall (A : LinDec) (m : A) (h h' : PairingHeap A),
+    isHeap h -> unT h = Some (m, h') -> size h = 1 + size h'.
+Proof.
+  destruct h; cbn; intros; inv H0.
+  rewrite mergePairs_size. reflexivity.
+Qed.
+
+Lemma unT_spec :
+  forall (A : LinDec) (m : A) (h h' : Tree A),
+    isHeap h -> unT h = Some (m, h') ->
+      forall x : A, elem x h -> m ≤ x.
+Proof.
+  destruct h; cbn; intros; inv H0.
+  inv H. induction H3; inv H1.
+    inv H0.
+    inv H2. inv H4.
+Qed.
+
+Lemma unT_elem_eq :
+  forall (A : LinDec) (m x : A) (h h' : Tree A),
+    isHeap h -> unT h = Some (m, h') ->
+      elem x h <-> x = m \/ elem x h'.
+Proof.
+  split.
+    destruct h; cbn; intros; inv H0.
+      inv H. induction H3; inv H1.
+        inv H0.
+        inv H2.
+          right. rewrite mergePairs_elem. auto.
+          inv H4. destruct (IHForall ltac:(auto) H6).
+            left. assumption.
+            right. rewrite mergePairs_elem in *. auto.
+    destruct 1; subst.
+      eapply unT_elem; eauto.
+      destruct h; cbn in *.
+        inv H0.
+        inv H0. constructor. rewrite mergePairs_elem in H1. auto.
+Qed.
+
+(** [toList] *)
+
+Function toList
+  {A : LinDec} (h : PairingHeap A) {measure size h}: list A :=
+match unT h with
+    | None => []
+    | Some (m, h') => m :: toList h'
+end.
+Proof.
+  destruct h; cbn; intros; subst; inv teq.
+    rewrite mergePairs_size. apply le_n.
+Defined.
+
+(*Lemma elem_toList_In :
+  forall (A : LinDec) (x : A) (h : PairingHeap A),
+    isHeap h -> elem x h <-> In x (toList h).
+Proof.
+  split; intros.
+    functional induction @toList A h; cbn.
+      destruct h; cbn in *.
+        inv H.
+        inv e.
+      assert (x = m \/ elem x h') by (eapply unT_elem_eq; eauto).
+        destruct H1; auto. apply unT_isHeap in e; auto.
+    functional induction @toList A h; cbn.
+      inv H0.
+      rewrite (@unT_elem_eq A m x h h'); auto.
+        apply unT_isHeap in e; auto. inv H0.
+Qed.*)
+
+Require Export Sorting.Sort.
+
+Theorem toList_sorted :
+  forall (A : LinDec) (h : PairingHeap A),
+    isHeap h -> sorted A (toList h).
+Proof.
+  intros. functional induction @toList A h.
+    constructor.
+    rewrite toList_equation in *. destruct h'; cbn in *; constructor.
+      eapply unT_spec; eauto. erewrite unT_elem_eq; eauto.
+      eapply IHl, unT_isHeap; eauto.
+Qed.
+
+(** [count_Tree] and its properties. *)
+Fixpoint countTree {A : LinDec} (x : A) (t : Tree A) : nat :=
+match t with
+    | E => 0
+    | T x' l =>
+        (if x =? x' then S else id)
+          (fold_right (fun h t => countTree x h + t) 0 l)
+end.
+
+Lemma countTree_empty :
+  forall (A : LinDec) (x : A),
+    countTree x empty = 0.
+Proof. reflexivity. Qed.
+
+Lemma countTree_singleton :
+  forall (A : LinDec) (x y : A),
+    countTree x (singleton y) = if x =? y then 1 else 0.
+Proof.
+  intros. dec.
+Qed.
+
+Lemma countTree_merge :
+  forall (A : LinDec) (x : A) (h1 h2 : PairingHeap A),
+    countTree x (merge h1 h2) = countTree x h1 + countTree x h2.
+Proof.
+  destruct h1, h2; cbn; intros; dec; dec; unfold id; omega.
+Qed.
+
+Lemma countTree_insert :
+  forall (A : LinDec) (x y : A) (h : PairingHeap A),
+    countTree x (insert y h) =
+      (if x =? y then S else id) (countTree x h).
+Proof.
+  intros. unfold insert. rewrite countTree_merge, countTree_singleton. dec.
+Qed.
+
+Lemma countTree_mergePairs :
+  forall (A : LinDec) (x : A) (l : list (PairingHeap A)),
+    countTree x (mergePairs l) =
+    fold_right (fun h t => countTree x h + t) 0 l.
+Proof.
+  intros. functional induction @mergePairs A l; cbn.
+    reflexivity.
+    rewrite <- plus_n_O. reflexivity.
+    rewrite !countTree_merge, IHp, plus_assoc. reflexivity.
+Qed.
+
+Lemma countTree_toList :
+  forall (A : LinDec) (x : A) (h : PairingHeap A),
+    isHeap h -> countTree x h = count A x (toList h).
+Proof.
+(*  induction h using Tree_ind_proper'; cbn; dec.
+    rewrite toList_equation. cbn. dec. f_equal.
+      induction l; cbn.
+      rewrite IHh, <- plus_n_O; auto. inv H0. inv H4.
+      inv H. rewrite H3, IHt. auto.*)
+  intros. functional induction @toList A h;
+  destruct h; inv e; cbn; dec.
+    rewrite <- IHl, countTree_mergePairs.
+      reflexivity.
+      apply mergePairs_isHeap. inv H.
+    rewrite <- IHl, countTree_mergePairs.
+      reflexivity.
+      apply mergePairs_isHeap. inv H.
+Qed.
+
+Fixpoint fromList {A : LinDec} (l : list A) : PairingHeap A :=
+match l with
+    | [] => E
+    | h :: t => insert h (fromList t)
+end.
+
+Lemma countTree_fromList :
+  forall (A : LinDec) (x : A) (l : list A),
+    countTree x (fromList l) = count A x l.
+Proof.
+  induction l as [| h t].
+    cbn. reflexivity.
+    unfold fromList. rewrite countTree_insert. fold fromList.
+      rewrite IHt. dec.
+Qed.
+
+Lemma fromList_isHeap :
+  forall (A : LinDec) (l : list A),
+    isHeap (fromList l).
+Proof.
+  induction l as [| h t].
+    cbn. constructor.
+    apply insert_isHeap. fold fromList. assumption.
+Qed.
+
+Definition pairingSort (A : LinDec) (l : list A) : list A :=
+  toList (fromList l).
+
+Theorem pairingSort_perm :
+  forall (A : LinDec) (l : list A),
+    perm A l (pairingSort A l).
+Proof.
+  unfold perm, pairingSort. intros.
+  rewrite <- countTree_toList, countTree_fromList.
+    reflexivity.
+    apply fromList_isHeap.
+Qed.
+
+Instance Sort_pairingSort : Sort :=
+{
+    sort := @pairingSort;
+}.
+Proof.
+  all: intros.
+    unfold pairingSort. apply toList_sorted, fromList_isHeap.
+    apply pairingSort_perm.
+Defined.
