DS/SplayHeap2.v
@@ -1,0 +1,357 @@
+Add Rec LoadPath "/home/zeimer/Code/Coq".
+
+Require Export BTree.
+Require Import BST.
+Require Export LinDec.
+Require Export Sorting.Sort.
+
+Set Implicit Arguments.
+
+Definition SplayHeap (A : LinDec) : Type := BTree A.
+
+Function bigger
+  {A : LinDec} (pivot : A) (h : SplayHeap A) : SplayHeap A :=
+match h with
+    | empty => empty
+    | node v l r =>
+        if v <=? pivot
+        then bigger pivot r
+        else
+          match l with
+              | empty => node v empty r
+              | node v' l' r' =>
+                  if v' <=? pivot
+                  then (* v' <= pivot < v *)
+                    node v (bigger pivot r') r
+                  else (* pivot < v' <= v *)
+                    node v' (bigger pivot l') (node v r' r)
+          end
+end.
+
+Compute bigger 2 (node 5 (node 2 empty empty) empty).
+
+Function smaller
+  {A : LinDec} (pivot : A) (h : SplayHeap A) : SplayHeap A :=
+match h with
+    | empty => empty
+    | node v l r =>
+        if v <=? pivot
+        then
+          match r with
+              | empty => node v l empty
+              | node v' l' r' =>
+                  if v' <=? pivot
+                  then (* v <= v' <= pivot *)
+                    node v' (node v l l') (smaller pivot r')
+                  else (* v <= pivot < v' *)
+                    node v l (smaller pivot l')
+          end
+        else smaller pivot l
+end.
+
+Compute smaller 4 (node 5 (node 2 empty empty) empty).
+
+Definition partition
+  {A : LinDec} (x : A) (h : SplayHeap A) : SplayHeap A * SplayHeap A:=
+    (smaller x h, bigger x h).
+
+Definition isEmpty
+  {A : LinDec} (h : SplayHeap A) : bool :=
+match h with
+    | empty => true
+    | _ => false
+end.
+
+Definition insert
+  {A : LinDec} (x : A) (h : SplayHeap A) : SplayHeap A :=
+    let (smaller, bigger) := partition x h
+    in node x smaller bigger.
+
+Function findMin
+  {A : LinDec} (h : SplayHeap A) : option A :=
+match h with
+    | empty => None
+    | node m empty _ => Some m
+    | node _ l _ => findMin l
+end.
+
+Function deleteMin
+  {A : LinDec} (h : SplayHeap A) : SplayHeap A :=
+match h with
+    | empty => empty
+    | node _ empty r => r
+    | node v l r => node v (deleteMin l) r
+end.
+
+Function deleteMin'
+  {A : LinDec} (h : SplayHeap A) : option A * SplayHeap A :=
+match h with
+    | empty => (None, empty)
+    | node m empty r => (Some m, r)
+    | node v l r =>
+        let '(min, l') := deleteMin' l in (min, node v l' r)
+end.
+
+Function merge {A : LinDec} (h1 h2 : SplayHeap A) : SplayHeap A :=
+match h1 with
+    | empty => h2
+    | node v l r =>
+        let '(l', r') := partition v h2
+        in node v (merge l l') (merge r r')
+end.
+
+(** Properties of [bigger] and [smaller]. *)
+
+Ltac aux := intros; repeat
+match goal with
+    | H : context [?x <=? ?y] |- _ =>
+        let H' := fresh "H" in
+          destruct (leqb_spec x y) as [H' | H']; try congruence;
+          clear H; rename H' into H
+    | H : ~ _ ≤ _ |- _ => destruct (LinDec_not_leq_lt _ _ _ H); clear H
+    | H : elem _ ?t, H' : forall _, elem _ ?t -> _ |- _ =>
+        specialize (H' _ H)
+    | H : ?a ≤ ?b, H' : ?b ≤ ?c |- ?a ≤ ?c =>
+        apply leq_trans with b; assumption
+    | H : elem _ empty |- _ => inv H
+    | H : elem _ (node _ _ _) |- _ => inv H
+    | H : is_bst ?x, H' : is_bst ?x -> _ |- _ => specialize (H' H)
+    | H : is_bst empty |- _ => inv H
+    | H : is_bst (node _ _ _) |- _ => inv H
+end; auto.
+
+(** Properties of [isEmpty] *)
+
+Lemma isEmpty_smaller_true :
+  forall (A : LinDec) (x : A) (h : SplayHeap A),
+    isEmpty h = true -> isEmpty (smaller x h) = true.
+Proof.
+  intros. functional induction @smaller A x h; cbn in *; aux.
+Qed.
+
+Lemma isEmpty_smaller_false :
+  forall (A : LinDec) (x : A) (h : SplayHeap A),
+    isEmpty (smaller x h) = false -> isEmpty h = false.
+Proof.
+  intros. functional induction @smaller A x h; cbn in *; aux.
+Qed.
+
+Lemma isEmpty_bigger_true :
+  forall (A : LinDec) (x : A) (h : SplayHeap A),
+    isEmpty h = true -> isEmpty (bigger x h) = true.
+Proof.
+  intros. functional induction @bigger A x h; cbn in *; aux.
+Qed.
+
+Lemma isEmpty_bigger_false :
+  forall (A : LinDec) (x : A) (h : SplayHeap A),
+    isEmpty (bigger x h) = false -> isEmpty h = false.
+Proof.
+  intros. functional induction @bigger A x h; cbn in *; aux.
+Qed.
+
+Lemma isEmpty_partition_true :
+  forall (A : LinDec) (x : A) (h l r : SplayHeap A),
+    partition x h = (l, r) ->
+      isEmpty h = true <-> isEmpty l = true /\ isEmpty r = true.
+Proof.
+  unfold partition. split; inv H; intros.
+    split.
+      apply isEmpty_smaller_true. assumption.
+      apply isEmpty_bigger_true. assumption.
+    destruct H.
+    induction h as [| v l IHl r IHr]; cbn in *.
+      reflexivity.
+      dec; [destruct r | destruct l]; dec.
+Qed.
+
+Lemma isEmpty_partition_false :
+  forall (A : LinDec) (x : A) (h l r : SplayHeap A),
+    partition x h = (l, r) ->
+      isEmpty h = false <-> isEmpty l = false \/ isEmpty r = false.
+Proof.
+  unfold partition. split; inv H; intros.
+    induction h as [| v l IHl r IHr]; cbn in *.
+      auto.
+      dec; [destruct r | destruct l]; dec.
+    destruct H.
+      eapply isEmpty_smaller_false. eassumption.
+      eapply isEmpty_bigger_false. eassumption.
+Qed.
+
+Lemma isEmpty_insert :
+  forall (A : LinDec) (x : A) (h : SplayHeap A),
+    isEmpty (insert x h) = false.
+Proof.
+  intros. unfold insert. case_eq (partition x h); intros small big H.
+  cbn. reflexivity.
+Qed.
+
+Lemma isEmpty_merge_true :
+  forall (A : LinDec) (h1 h2 : SplayHeap A),
+    isEmpty (merge h1 h2) = true <->
+      isEmpty h1 = true /\ isEmpty h2 = true.
+Proof.
+  destruct h1; cbn; intros; try destruct (partition c h2); firstorder.
+Qed.
+
+Lemma isEmpty_merge_false :
+  forall (A : LinDec) (h1 h2 : SplayHeap A),
+    isEmpty (merge h1 h2) = false <->
+      isEmpty h1 = false \/ isEmpty h2 = false.
+Proof.
+  destruct h1; cbn; intros; try destruct (partition c h2); firstorder.
+Qed.
+
+(** Properties [bigger]. *)
+
+Lemma bigger_spec :
+  forall (A : LinDec) (pivot : A) (h : SplayHeap A),
+    is_bst h -> forall x : A, elem x (bigger pivot h) ->
+      pivot ≤ x /\ pivot <> x.
+Proof.
+  intros. functional induction @bigger A pivot h; aux;
+  (split; [eauto | intro; subst; dec]).
+Qed.
+
+Lemma bigger_elem :
+  forall (A : LinDec) (x pivot : A) (h : SplayHeap A),
+    is_bst h -> elem x (bigger pivot h) -> elem x h.
+Proof.
+  intros. functional induction @bigger A pivot h; aux.
+Qed.
+
+Lemma bigger_elem' :
+  forall (A : LinDec) (x pivot : A) (h : SplayHeap A),
+    is_bst h -> elem x h -> pivot ≤ x -> pivot <> x ->
+      elem x (bigger pivot h).
+Proof.
+  intros. functional induction @bigger A pivot h; aux;
+  contradiction H2; dec.
+Qed.
+
+Lemma bigger_is_bst :
+  forall (A : LinDec) (pivot : A) (h : SplayHeap A),
+    is_bst h -> is_bst (bigger pivot h).
+Proof.
+  intros. functional induction @bigger A pivot h; aux.
+    repeat constructor; auto; intros. apply bigger_elem in H; auto.
+    repeat constructor; auto; intros.
+      apply bigger_elem in H; auto.
+      inv H. eauto.
+Qed.
+
+(** Properties of [smaller]. *)
+Lemma smaller_spec :
+  forall (A : LinDec) (pivot : A) (h h' : SplayHeap A),
+    is_bst h -> smaller pivot h = h' ->
+      forall x : A, elem x h' -> x ≤ pivot.
+Proof.
+  intros. functional induction @smaller A pivot h; aux; eauto.
+Qed.
+
+Lemma smaller_elem :
+  forall (A : LinDec) (x pivot : A) (h : SplayHeap A),
+    is_bst h -> elem x (smaller pivot h) -> elem x h.
+Proof.
+  intros. functional induction @smaller A pivot h; aux.
+Qed.
+
+Lemma smaller_elem' :
+  forall (A : LinDec) (x pivot : A) (h : SplayHeap A),
+    is_bst h -> elem x h -> x ≤ pivot ->
+      elem x (smaller pivot h).
+Proof.
+  intros. functional induction @smaller A pivot h; aux;
+  contradiction H3; dec.
+Qed.
+
+Lemma smaller_is_bst :
+  forall (A : LinDec) (pivot : A) (h : SplayHeap A),
+    is_bst h -> is_bst (smaller pivot h).
+Proof.
+  intros. functional induction @smaller A pivot h; aux.
+    repeat constructor; auto; intros.
+      inv H. eauto.
+      apply smaller_elem in H; auto.
+    repeat constructor; auto; intros. apply smaller_elem in H; auto.
+Qed.
+
+(** Properties of [partition]. *)
+
+Lemma partition_elem :
+  forall (A : LinDec) (x pivot : A) (h l r : SplayHeap A),
+    is_bst h -> partition pivot h = (l, r) ->
+      elem x h <-> elem x l \/ elem x r.
+Proof.
+  intros. inv H0. split; intros.
+    destruct (leqb_spec x pivot).
+      left. eapply smaller_elem'; aux.
+      right. eapply bigger_elem'; aux.
+    destruct H0.
+      eapply smaller_elem; eauto.
+      eapply bigger_elem; eauto.
+Qed.
+
+Lemma partition_is_bst :
+  forall (A : LinDec) (x : A) (h l r : SplayHeap A),
+    partition x h = (l, r) -> is_bst h -> is_bst (node x l r).
+Proof.
+  unfold partition. inversion 1; subst; clear H. constructor.
+    eapply smaller_spec; eauto.
+    apply smaller_is_bst. assumption.
+    eapply bigger_spec; eauto.
+    apply bigger_is_bst. assumption.
+Qed.
+
+(** Properties of [insert]. *)
+Lemma insert_elem :
+  forall (A : LinDec) (x : A) (h : SplayHeap A),
+    elem x (insert x h).
+Proof.
+  intros. unfold insert. destruct (partition x h). constructor.
+Qed.
+
+Lemma insert_is_bst :
+  forall (A : LinDec) (x : A) (h : SplayHeap A),
+    is_bst h -> is_bst (insert x h).
+Proof.
+  intros. unfold insert. case_eq (partition x h); intros l r H'.
+  eapply partition_is_bst; eauto.
+Qed.
+
+(** Properties of [merge]. *)
+
+Lemma merge_elem :
+  forall (A : LinDec) (x : A) (h1 h2 : SplayHeap A),
+    is_bst h1 -> is_bst h2 ->
+      elem x (merge h1 h2) <-> elem x h1 \/ elem x h2.
+Proof.
+  split; intros.
+    functional induction @merge A h1 h2; intros.
+      right. assumption.
+      assert (is_bst (node v l' r')) by (eapply partition_is_bst; eauto).
+        aux; inv e0.
+          destruct (IHs _ H10 H7 H4); aux. right.
+            eapply smaller_elem; eauto.
+          destruct (IHs0 _ H12 H9 H4); aux. right.
+            eapply bigger_elem; eauto.
+    functional induction @merge A h1 h2; intros.
+      inv H1; inv H2.
+      inv H. inv H1.
+        apply partition_is_bst in e0; inv e0. inv H.
+        rewrite partition_elem in H; eauto.
+          apply partition_is_bst in e0; inv H; eauto.
+Qed.
+
+Lemma merge_is_bst :
+  forall (A : LinDec) (h1 h2 : SplayHeap A),
+    is_bst h1 -> is_bst h2 -> is_bst (merge h1 h2).
+Proof.
+  induction h1 as [| v l IHl r IHr]; intros.
+    assumption.
+    unfold merge. case_eq (partition v h2); intros small big Hp; fold merge.
+      apply partition_is_bst in Hp; aux. constructor; intros; auto.
+        apply merge_elem in H; firstorder.
+        apply merge_elem in H; firstorder.
+Qed.
