Reflection/Reflection_a_la_carte.v
@@ -2,7 +2,7 @@ Add Rec LoadPath "/home/zeimer/Code/Coq".
 
 Require Export RCCBase.
 Require Import HSLib.Base.
-Require Import HSLib.Functor.Functor.
+Require Import HSLib.Control.Functor.
 
 Set Implicit Arguments.
 
