Sorting/Heapsort.v
@@ -1,16 +1,14 @@
 Add Rec LoadPath "/home/zeimer/Code/Coq".
 
-Require Export Coq.Program.Wf.
-Require Export Recdef.
+Require Import RCCBase.
 
 Require Export Sorting.Sort.
 Require Export ListLemmas.
 
 Require Export BTree.
 Require Export BST.
-Require Export LeftistHeap.
 
-Set Implicit Arguments.
+Require Import LeftistHeap.
 
 (* Leftist heapsort *)
 Function fromList {A : LinDec} (l : list A) : BTree A :=
